# 15.1-1

T(0) = 1
T(n) = 1 + sum(T(j)) (j in [0, n - 1])

---

1. T(0) = 2 ^ 0 = 1
2. T(0),..,T(n-1)
=> T(n) = 1 + (1 + 2^1 + .. + 2^(n-1))
        = 2 + 2^1 + .. + 2^(n-1)
        = 2^n

# 15.1-2

# 15.1-3

check CutRod.hs

N    | 1 | 2 | 3 | 4  | 5  | 6  | 7  | 8  | 9  | 10 |
-----|---|---|---|----|----|----|----|----|----|----|
p    | 1 | 5 | 8 | 9  | 10 | 17 | 17 | 20 | 24 | 30 |
c=0  | 1 | 5 | 8 | 10 | 13 | 17 | 18 | 22 | 25 | 30 |
c=1  | 1 | 5 | 8 | 9  | 10 | 17 | 17 | 20 | 24 | 30 |

# 15.1-4

check CutRod.hs

# 15.1-5

fib
